src/tls/TLSConstants.fst
@@ -176,8 +176,8 @@ type signatureScheme =
   | RSA_PSS_SHA384
   | RSA_PSS_SHA512
   // EdDSA algorithms
-  //| ED25519
-  //| ED448
+  //  | ED25519_SHA512
+  //  | ED448_SHAKE256
   // Legacy algorithms
   | RSA_PKCS1_SHA1
   | RSA_PKCS1_MD5SHA1 // Only used internally, with codepoint 0xFFFF (PRIVATE_USE)
@@ -187,22 +187,20 @@ type signatureScheme =
   | DSA_SHA256
   | DSA_SHA384
   | DSA_SHA512
-  | OBSOLETE of (codepoint:lbytes 2 {
+  | SIG_UNKNOWN of (codepoint: lbytes 2 {
       let v = int_of_bytes codepoint in
-      (0x0000 <= v /\ v <= 0x0100) \/
-      (0x0204 <= v /\ v <= 0x0400) \/
-      (0x0404 <= v /\ v <= 0x0500) \/
-      (0x0504 <= v /\ v <= 0x0600) \/
-      (0x0604 <= v /\ v <= 0x06FF) })
-  | PRIVATE_USE of (codepoint:lbytes 2 {
-      let v = int_of_bytes codepoint in 0xFE00 <= v /\ v < 0xFFFF})
+          v <> 0x0401 /\ v <> 0x0501 /\ v <> 0x0601 /\ v <> 0x0403
+       /\ v <> 0x0503 /\ v <> 0x0603 /\ v <> 0x0804 /\ v <> 0x0805
+       /\ v <> 0x0806 /\ v <> 0x0807 /\ v <> 0x0808 /\ v <> 0x0201
+       /\ v <> 0x0203 /\ v <> 0x0202 /\ v <> 0x0402 /\ v <> 0x0502
+       /\ v <> 0x0602})
 
 let is_handshake13_signatureScheme = function
   | ECDSA_SECP256R1_SHA256
   | ECDSA_SECP384R1_SHA384
   | ECDSA_SECP521R1_SHA512
-//| ED25519
-//| ED448
+  //| ED25519_SHA512
+  //| ED448_SHAKE256
   | RSA_PSS_SHA256
   | RSA_PSS_SHA384
   | RSA_PSS_SHA512 -> true
@@ -219,8 +217,8 @@ let signatureSchemeBytes = function
   | RSA_PSS_SHA256         -> abyte2 (0x08z, 0x04z)
   | RSA_PSS_SHA384         -> abyte2 (0x08z, 0x05z)
   | RSA_PSS_SHA512         -> abyte2 (0x08z, 0x06z)
-  //| ED25519                -> abyte2 (0x08z, 0x07z)
-  //| ED448                  -> abyte2 (0x08z, 0x08z)
+  //| ED25519_SHA512         -> abyte2 (0x08z, 0x07z)
+  //| ED448_SHAKE256         -> abyte2 (0x08z, 0x08z)
   | RSA_PKCS1_SHA1         -> abyte2 (0x02z, 0x01z)
   | RSA_PKCS1_MD5SHA1      -> abyte2 (0xFFz, 0xFFz)
   | ECDSA_SHA1             -> abyte2 (0x02z, 0x03z)
@@ -228,15 +226,14 @@ let signatureSchemeBytes = function
   | DSA_SHA256             -> abyte2 (0x04z, 0x02z)
   | DSA_SHA384             -> abyte2 (0x05z, 0x02z)
   | DSA_SHA512             -> abyte2 (0x06z, 0x02z)
-  | OBSOLETE codepoint     -> codepoint
-  | PRIVATE_USE codepoint  -> codepoint
+  | SIG_UNKNOWN codepoint  -> codepoint
 
 let signatureSchemeBytes_is_injective
   (s1 s2: signatureScheme)
 : Lemma
   (requires (Seq.equal (signatureSchemeBytes s1) (signatureSchemeBytes s2)))
   (ensures (s1 == s2))
-= if (OBSOLETE? s1 || PRIVATE_USE? s1) = (OBSOLETE? s2 || PRIVATE_USE? s2)
+= if (SIG_UNKNOWN? s1) = (SIG_UNKNOWN? s2)
   then ()
   else assume (s1 == s2) // TODO: strengthen int_of_bytes vs. abyte2
 
@@ -252,8 +249,8 @@ let parseSignatureScheme b =
   | (0x08z, 0x04z) -> Correct RSA_PSS_SHA256
   | (0x08z, 0x05z) -> Correct RSA_PSS_SHA384
   | (0x08z, 0x06z) -> Correct RSA_PSS_SHA512
-  //| (0x08z, 0x07z) -> Correct ED25519
-  //| (0x08z, 0x08z) -> Correct ED448
+  //| (0x08z, 0x07z) -> Correct ED25519_SHA512
+  //| (0x08z, 0x08z) -> Correct ED448_SHAKE256
   | (0x02z, 0x01z) -> Correct RSA_PKCS1_SHA1
   | (0xFFz, 0xFFz) -> Correct RSA_PKCS1_MD5SHA1
   | (0x02z, 0x03z) -> Correct ECDSA_SHA1
@@ -261,19 +258,10 @@ let parseSignatureScheme b =
   | (0x04z, 0x02z) -> Correct DSA_SHA256
   | (0x05z, 0x02z) -> Correct DSA_SHA384
   | (0x06z, 0x02z) -> Correct DSA_SHA512
-  | (x, y) ->
-     let v = int_of_bytes b in
-     if (0x0000 <= v && v <= 0x0100) ||
-        (0x0204 <= v && v <= 0x0400) ||
-        (0x0404 <= v && v <= 0x0500) ||
-        (0x0504 <= v && v <= 0x0600) ||
-        (0x0604 <= v && v <= 0x06FF)
-     then Correct (OBSOLETE b)
-     else if 0xFE00 <= v && v < 0xFFFF then Correct (PRIVATE_USE b)
-     else Error(AD_decode_error, "Parsed invalid SignatureScheme " ^ print_bytes b)
+  | (x, y) -> Correct (SIG_UNKNOWN b)
 
 val sigHashAlg_of_signatureScheme:
-  scheme:signatureScheme{~(PRIVATE_USE? scheme) /\ ~(OBSOLETE? scheme)} -> sigAlg * hashAlg
+  scheme:signatureScheme{~(SIG_UNKNOWN? scheme)} -> sigAlg * hashAlg
 let sigHashAlg_of_signatureScheme =
   let open CoreCrypto in
   let open Hashing.Spec in
@@ -287,9 +275,9 @@ let sigHashAlg_of_signatureScheme =
   | RSA_PSS_SHA256         -> (RSAPSS, Hash SHA256)
   | RSA_PSS_SHA384         -> (RSAPSS, Hash SHA384)
   | RSA_PSS_SHA512         -> (RSAPSS, Hash SHA512)
-  //| ED25519                -> (EdDSA,  Hash SHA512)
-  //| ED448                  -> (EdDSA,  Hash SHA512)
-  | RSA_PKCS1_SHA1         -> (RSASIG,    Hash SHA1)
+//  | ED25519_SHA512         -> (EdDSA,  Hash SHA512)
+//  | ED448_SHAKE256         -> (EdDSA,  Hash SHAKE256)
+  | RSA_PKCS1_SHA1         -> (RSASIG, Hash SHA1)
   | RSA_PKCS1_MD5SHA1      -> (RSASIG, MD5SHA1)
   | ECDSA_SHA1             -> (ECDSA,  Hash SHA1)
   | DSA_SHA1               -> (DSA,    Hash SHA1)
@@ -311,8 +299,8 @@ let signatureScheme_of_sigHashAlg sa ha =
   | (RSAPSS, Hash SHA256) -> RSA_PSS_SHA256
   | (RSAPSS, Hash SHA384) -> RSA_PSS_SHA384
   | (RSAPSS, Hash SHA512) -> RSA_PSS_SHA512
-  //| ED25519               -> (EdDSA,  Hash SHA512)
-  //| ED448                 -> (EdDSA,  Hash SHA512)
+  //| (EdDSA,  Hash SHA512) -> ED25519_SHA512
+  //| (EdDSA,  Hash SHAKE256) -> ED448_SHAKE256
   | (RSASIG, Hash SHA1)   -> RSA_PKCS1_SHA1
   | (ECDSA,  Hash SHA1)   -> ECDSA_SHA1
   | (DSA,    Hash SHA1)   -> DSA_SHA1
@@ -322,7 +310,7 @@ let signatureScheme_of_sigHashAlg sa ha =
   | (RSASIG, MD5SHA1)     -> RSA_PKCS1_MD5SHA1
   | _ -> // Map everything else to OBSOLETE 0x0000
     lemma_repr_bytes_values 0x0000; int_of_bytes_of_int 2 0x0000;
-    OBSOLETE (bytes_of_int 2 0x0000)
+    SIG_UNKNOWN (bytes_of_int 2 0)
 
 (** Encryption key sizes *)
 let encKeySize =
@@ -482,10 +470,10 @@ val pinverse_version: x:_ -> Lemma
   [SMTPat (versionBytes (Correct?._0 (parseVersion x)))]
 let pinverse_version x = ()
 
-// DRAFT#20
+// DRAFT#21
 // to be used *only* in ServerHello.version.
 // https://tlswg.github.io/tls13-spec/#rfc.section.4.2.1
-let draft = 20z
+let draft = 21z
 let versionBytes_draft: protocolVersion -> Tot (lbytes 2) = function
   | TLS_1p3 -> abyte2 ( 127z, draft )
   | pv -> versionBytes pv
@@ -1755,21 +1743,21 @@ type quicParameters =
 let string_of_quicVersion = function
   | QuicVersion1 -> "v1"
   | QuicCustomVersion n -> "v"^UInt32.to_string n
-let string_of_quicParameter = function 
+let string_of_quicParameter = function
   | Quic_initial_max_stream_data x -> "initial_max_stream_data="^UInt32.to_string x
   | Quic_initial_max_data x -> "initial_max_data="^UInt32.to_string x
   | Quic_initial_max_stream_id x -> "initial_max_stream="^UInt32.to_string x
   | Quic_idle_timeout x -> "idle_timeout="^UInt16.to_string x
   | Quic_truncate_connection_id -> "truncate_connection_id"
-  | Quic_max_packet_size x -> "max_packet_size="^UInt16.to_string x 
+  | Quic_max_packet_size x -> "max_packet_size="^UInt16.to_string x
   | Quic_custom_parameter (n,b) -> "custom_parameter "^UInt16.to_string n^", "^print_bytes b
 let string_of_quicParameters = function
-  | Some (QuicParametersClient n i p)  -> 
+  | Some (QuicParametersClient n i p)  ->
     "QUIC client parameters\n" ^
     "negotiated version: "^string_of_quicVersion n^"\n"^
     "initial version: "^string_of_quicVersion i^"\n"^
     List.Tot.fold_left (fun a p -> a^string_of_quicParameter p^"\n") "" p
-  | Some (QuicParametersServer v p) -> 
+  | Some (QuicParametersServer v p) ->
     "QUIC server parameters\n" ^
     List.Tot.fold_left (fun a v -> a^string_of_quicVersion v^" ") "versions: " v ^ "\n" ^
     List.Tot.fold_left (fun a p -> a^string_of_quicParameter p^"\n") "" p
